src/PlutusIR/Semantics/SemanticEquivalence/FundamentalProperty.v
@@ -76,7 +76,7 @@ Proof with eauto.
       * simpl. destruct t0. simpl.
         unfold inclusion.
         intros.
-        destruct (s =? x)%string eqn:Heqb.
+        destruct (b =? x)%string eqn:Heqb.
         -- eapply eqb_eq in Heqb as Heq.
            subst.
            assert (appears_bound_in_ann x (Let NonRec (TypeBind (TyVarDecl x k) t1 :: bs) t)) by eauto.
@@ -90,10 +90,10 @@ Proof with eauto.
         simpl.
         unfold inclusion.
         intros.
-        destruct (s0 =? x)%string eqn:Heqb.
+        destruct (b0 =? x)%string eqn:Heqb.
         -- eapply eqb_eq in Heqb as Heq.
            subst.
-           assert (appears_bound_in_ann x (Let NonRec (DatatypeBind (Datatype (TyVarDecl x k) l s l0) :: bs) t)) by eauto.
+           assert (appears_bound_in_ann x (Let NonRec (DatatypeBind (Datatype (TyVarDecl x k) l b l0) :: bs) t)) by eauto.
            eapply uniqueness' in H4.
            rewrite H4 in H1.
            inversion H4.
